Test/dafny1/UltraFilter.dfy
@@ -3,109 +3,100 @@
 
 // ultra filter
 
-class UltraFilter<G(==)> {
-  static function IsFilter(f: set<set<G>>, S: set<G>): bool
-  {
-    (forall A, B :: A in f && A <= B ==> B in f) &&
-    (forall C, D :: C in f && D in f ==> C * D in f) &&
-    S in f &&
-    {} !in f
-  }
+type G(==)
 
-  static function IsUltraFilter(f: set<set<G>>, S: set<G>): bool
-  {
-    IsFilter(f, S) &&
-    (forall g :: IsFilter(g, S) && f <= g ==> f == g)
-  }
+predicate IsFilter(f: set<set<G>>, S: set<G>)
+{
+  (forall A, B :: A in f && A <= B ==> B in f) &&
+  (forall C, D :: C in f && D in f ==> C * D in f) &&
+  S in f &&
+  {} !in f
+}
 
-  method Theorem(f: set<set<G>>, S: set<G>, M: set<G>, N: set<G>)
-    requires IsUltraFilter(f, S);
-    requires M + N in f;
-    ensures M in f || N in f;
-  {
-    if (M !in f) {
-      // instantiate 'g' with the following 'h'
-      var h := H(f, S, M);
-      Lemma_HIsFilter(h, f, S, M);
-      Lemma_FHOrdering0(h, f, S, M);
+predicate IsUltraFilter(f: set<set<G>>, S: set<G>)
+{
+  IsFilter(f, S) &&
+  (forall g :: IsFilter(g, S) && f <= g ==> f == g)
+}
+
+lemma Theorem(f: set<set<G>>, S: set<G>, M: set<G>, N: set<G>)
+  requires IsUltraFilter(f, S)
+  requires M + N in f
+  ensures M in f || N in f
+{
+  if M !in f {
+    // instantiate 'g' with the following 'h'
+    var h := H(f, S, M);
+    Lemma_HIsFilter(h, f, S, M);
+    Lemma_FHOrdering(h, f, S, M);
+  }
+}
+
+// H is really just a name for a set comprehension
+lemma H(f: set<set<G>>, S: set<G>, M: set<G>) returns (h: set<set<G>>)
+  ensures forall X :: X in h <==> M + X in f
+{
+  h := set X,Y | Y in f && X <= Y && M + X == Y :: X;
+  forall X {
+    calc {
+      X in h;
+      exists Y :: Y in f && X <= Y && M + X == Y;
+      M + X in f;
     }
   }
+}
 
-  // Dafny currently does not have a set comprehension expression, so this method stub will have to do
-  method H(f: set<set<G>>, S: set<G>, M: set<G>) returns (h: set<set<G>>)
-    ensures (forall X :: X in h <==> M + X in f);
-
-  method Lemma_HIsFilter(h: set<set<G>>, f: set<set<G>>, S: set<G>, M: set<G>)
-    requires IsFilter(f, S);
-    requires (forall X :: X in h <==> M + X in f);
-    requires M !in f;
-    ensures IsFilter(h, S);
-  {
-    // call Lemma_H0(h, f, S, M, *, *);
-    assume (forall A, B :: A in h && A <= B ==> B in h);
-
-    // call Lemma_H1(h, f, S, M, *, *);
-    assume (forall C, D :: C in h && D in h ==> C * D in h);
-
-    Lemma_H2(h, f, S, M);
-
-    Lemma_H3(h, f, S, M);
-  }
-
-  method Lemma_H0(h: set<set<G>>, f: set<set<G>>, S: set<G>, M: set<G>, A: set<G>, B: set<G>)
-    requires IsFilter(f, S);
-    requires (forall X :: X in h <==> M + X in f);
-    requires A in h && A <= B;
-    ensures B in h;
+lemma Lemma_HIsFilter(h: set<set<G>>, f: set<set<G>>, S: set<G>, M: set<G>)
+  requires IsFilter(f, S)
+  requires forall X :: X in h <==> M + X in f
+  requires M !in f
+  ensures IsFilter(h, S)
+{
+  forall A, B | A in h && A <= B
+    ensures B in h
   {
     assert M + A <= M + B;
   }
 
-  method Lemma_H1(h: set<set<G>>, f: set<set<G>>, S: set<G>, M: set<G>, C: set<G>, D: set<G>)
-    requires IsFilter(f, S);
-    requires (forall X :: X in h <==> M + X in f);
-    requires C in h && D in h;
-    ensures C * D in h;
+  forall C, D | C in h && D in h
+    ensures C * D in h
   {
     assert (M + C) * (M + D) == M + (C * D);
   }
 
-  method Lemma_H2(h: set<set<G>>, f: set<set<G>>, S: set<G>, M: set<G>)
-    requires IsFilter(f, S);
-    requires (forall X :: X in h <==> M + X in f);
-    ensures S in h;
-  {
-    // S is intended to stand for the universal set, but this is the only place where that plays a role
-    assume M <= S;
+  Lemma_H2(h, f, S, M);
 
-    assert M + S == S;
-  }
+  Lemma_H3(h, f, S, M);
+}
 
-  method Lemma_H3(h: set<set<G>>, f: set<set<G>>, S: set<G>, M: set<G>)
-    requires IsFilter(f, S);
-    requires (forall X :: X in h <==> M + X in f);
-    requires M !in f;
-    ensures {} !in h;
-  {
-    assert M + {} == M;
-  }
+lemma Lemma_H2(h: set<set<G>>, f: set<set<G>>, S: set<G>, M: set<G>)
+  requires IsFilter(f, S)
+  requires forall X :: X in h <==> M + X in f
+  ensures S in h
+{
+  // S is intended to stand for the universal set, but this is the only place where that plays a role
+  assume M <= S;
 
-  method Lemma_FHOrdering0(h: set<set<G>>, f: set<set<G>>, S: set<G>, M: set<G>)
-    requires IsFilter(f, S);
-    requires (forall X :: X in h <==> M + X in f);
-    requires IsFilter(h, S);
-    ensures f <= h;
-  {
-    // call Lemma_FHOrdering1(h, f, S, M, *);
-    assume (forall Y :: Y in f ==> Y in h);
-    assume f <= h;  // hickup in boxing
-  }
+  assert M + S == S;
+}
 
-  method Lemma_FHOrdering1(h: set<set<G>>, f: set<set<G>>, S: set<G>, M: set<G>, Y: set<G>)
-    requires IsFilter(f, S);
-    requires (forall X :: X in h <==> M + X in f);
-    ensures Y in f ==> Y in h;
+lemma Lemma_H3(h: set<set<G>>, f: set<set<G>>, S: set<G>, M: set<G>)
+  requires IsFilter(f, S)
+  requires forall X :: X in h <==> M + X in f
+  requires M !in f
+  ensures {} !in h
+{
+  assert M + {} == M;
+}
+
+lemma Lemma_FHOrdering(h: set<set<G>>, f: set<set<G>>, S: set<G>, M: set<G>)
+  requires IsFilter(f, S)
+  requires forall X :: X in h <==> M + X in f
+  requires IsFilter(h, S)
+  ensures f <= h
+{
+  forall Y | Y in f
+    ensures Y in h
   {
-    assert Y <= M + Y;
   }
 }
