Test/hofs/Field.dfy
@@ -4,20 +4,19 @@
 // calling fields should not make a resolution error:
 
 class Ref<A(0)> {
-  var val: A;
+  var val: A
 }
 
 method Nope() {
-  var f := new Ref<int -> bool>;
-  assert f.val(0);
+  var f := new Ref<int --> bool>;
+  assert f.val(0);  // error: precondition and assert
 }
 
 class FnRef<A(0),B(0)> {
-  var fn: A -> B;
+  var fn: A --> B
 }
 
 method Nope2() {
   var f := new FnRef<int,bool>;
-  assert f.fn(0);
+  assert f.fn(0);  // error: precondition and assert
 }
-
