Test/hofs/Fold.dfy
@@ -8,18 +8,17 @@ datatype Expr = Add(List<Expr>) | Mul(List<Expr>) | Lit(int)
 function method Eval(e : Expr): int
 {
   match e
-    case Add(es) => Fold(es,0,(e,v) requires e < es => Eval(e) + v)
-    case Mul(es) => Fold(es,1,(e,v) requires e < es => Eval(e) * v)
+    case Add(es) => Fold(es, 0, (e,v) requires e < es => Eval(e) + v)
+    case Mul(es) => Fold(es, 1, (e,v) requires e < es => Eval(e) * v)
     case Lit(i)  => i
 }
 
-function method Fold<A,B>(xs : List<A>, unit : B, f : (A,B) -> B): B
-  reads f.reads;
-  requires forall x, y :: x < xs ==> f.requires(x,y);
+function method Fold<A,B>(xs : List<A>, unit : B, f : (A,B) --> B): B
+  requires forall x, y :: x < xs ==> f.requires(x,y)
 {
   match xs
     case Nil => unit
-    case Cons(x,xs) => f(x,Fold(xs,unit,f))
+    case Cons(x,xs) => f(x, Fold(xs, unit, f))
 }
 
 method Main() {
