Test/hofs/ReadsReads.dfy
@@ -2,58 +2,58 @@
 // RUN: %diff "%s.expect" "%t"
 
 module ReadsRequiresReads {
-  function MyReadsOk<A,B>(f : A -> B, a : A) : set<object>
+  function MyReadsOk<A,B>(f : A ~> B, a : A) : set<object>
     reads f.reads(a)
   {
     f.reads(a)
   }
 
-  function MyReadsOk2<A,B>(f : A -> B, a : A) : set<object>
+  function MyReadsOk2<A,B>(f : A ~> B, a : A) : set<object>
     reads f.reads(a)
   {
     (f.reads)(a)
   }
 
-  function MyReadsOk3<A,B>(f : A -> B, a : A) : set<object>
+  function MyReadsOk3<A,B>(f : A ~> B, a : A) : set<object>
     reads (f.reads)(a)
   {
     f.reads(a)
   }
 
-  function MyReadsOk4<A,B>(f : A -> B, a : A) : set<object>
+  function MyReadsOk4<A,B>(f : A ~> B, a : A) : set<object>
     reads (f.reads)(a)
   {
     (f.reads)(a)
   }
 
-  function MyReadsBad<A,B>(f : A -> B, a : A) : set<object>
+  function MyReadsBad<A,B>(f : A ~> B, a : A) : set<object>
   {
     f.reads(a)  // error: MyReadsBad does not have permission to read what f.reads(a) reads
   }
 
-  function MyReadsBad2<A,B>(f : A -> B, a : A) : set<object>
+  function MyReadsBad2<A,B>(f : A ~> B, a : A) : set<object>
   {
     (f.reads)(a)  // error: MyReadsBad2 does not have permission to read what f.reads(a) reads
   }
 
-  function MyReadsOk'<A,B>(f : A -> B, a : A, o : object) : bool
+  function MyReadsOk'<A,B>(f : A ~> B, a : A, o : object) : bool
     reads f.reads(a)
   {
     o in f.reads(a)
   }
 
-  function MyReadsBad'<A,B>(f : A -> B, a : A, o : object) : bool
+  function MyReadsBad'<A,B>(f : A ~> B, a : A, o : object) : bool
   {
     o in f.reads(a)  // error: MyReadsBad' does not have permission to read what f.reads(a) reads
   }
 
-  function MyRequiresOk<A,B>(f : A -> B, a : A) : bool
+  function MyRequiresOk<A,B>(f : A ~> B, a : A) : bool
     reads f.reads(a)
   {
     f.requires(a)
   }
 
-  function MyRequiresBad<A,B>(f : A -> B, a : A) : bool
+  function MyRequiresBad<A,B>(f : A ~> B, a : A) : bool
   {
     f.requires(a)  // error: MyRequiresBad does not have permission to read what f.requires(a) reads
   }
@@ -104,28 +104,28 @@ module WhatWeKnowAboutReads {
 }
 
 module ReadsAll {
-  function A(f: int -> int) : int
+  function A(f: int ~> int) : int
     reads set x,o | o in f.reads(x) :: o  // note, with "set o,x ..." instead, Dafny complains (this is perhaps less than ideal)
     requires forall x :: f.requires(x)
   {
     f(0) + f(1) + f(2)
   }
 
-  function method B(f: int -> int) : int
+  function method B(f: int ~> int) : int
     reads set x,o | o in f.reads(x) :: o  // note, with "set o,x ..." instead, Dafny complains (this is perhaps less than ideal)
     requires forall x :: f.requires(x)
   {
     f(0) + f(1) + f(2)
   }
 
-  function C(f: int -> int) : int
+  function C(f: int ~> int) : int
     reads f.reads
     requires forall x :: f.requires(x)
   {
     f(0) + f(1) + f(2)
   }
 
-  function method D(f: int -> int) : int
+  function method D(f: int ~> int) : int
     reads f.reads
     requires forall x :: f.requires(x)
   {
@@ -134,7 +134,7 @@ module ReadsAll {
 }
 
 module ReadsOnFunctions {
-  lemma Requires_Reads_What_Function_Reads(f: int -> int)
+  lemma Requires_Reads_What_Function_Reads(f: int ~> int)
   {
     var g := f.requires;
     assert g.reads(10) == f.reads(10);
