Test/hofs/SumSum.dfy
@@ -5,57 +5,57 @@
 // Many of these currently require far more effort than one would like.
 // KRML, 2 May 2016
 
-predicate Total<X,R>(f: X -> R)
+predicate Total<X,R>(f: X ~> R)
   reads f.reads
 {
   forall x :: f.reads(x) == {} && f.requires(x)
 }
 
-predicate Total2<X,Y,R>(f: (X,Y) -> R)
+predicate Total2<X,Y,R>(f: (X,Y) ~> R)
   reads f.reads
 {
   forall x,y :: f.reads(x,y) == {} && f.requires(x,y)
 }
 
-function Sum(n: nat, f: int -> int): int
+function Sum(n: nat, f: int ~> int): int
   requires Total(f)
 {
   if n == 0 then 0 else f(n-1) + Sum(n-1, f)
 }
 
-lemma Exchange(n: nat, f: int -> int, g: int -> int)
+lemma Exchange(n: nat, f: int ~> int, g: int ~> int)
   requires Total(f) && Total(g)
   requires forall i :: 0 <= i < n ==> f(i) == g(i)
   ensures Sum(n, f) == Sum(n, g)
 {
 }
 
-lemma ExchangeEta(n: nat, f: int -> int, g: int -> int)
+lemma ExchangeEta(n: nat, f: int ~> int, g: int ~> int)
   requires Total(f) && Total(g)
   requires forall i :: 0 <= i < n ==> f(i) == g(i)
   ensures Sum(n, x => f(x)) == Sum(n, x => g(x))
 {
 }
   
-lemma NestedAlphaRenaming(n: nat, g: (int,int) -> int)
+lemma NestedAlphaRenaming(n: nat, g: (int,int) ~> int)
   requires Total2(g)
   ensures Sum(n, x => Sum(n, y => g(x,y))) == Sum(n, a => Sum(n, b => g(a,b)))
 {
 }
 
-lemma DistributePlus1(n: nat, f: int -> int)
+lemma DistributePlus1(n: nat, f: int ~> int)
   requires Total(f)
   ensures Sum(n, x => 1 + f(x)) == n + Sum(n, f)
 {
 }
 
-lemma Distribute(n: nat, f: int -> int, g: int -> int)
+lemma Distribute(n: nat, f: int ~> int, g: int ~> int)
   requires Total(f) && Total(g)
   ensures Sum(n, x => f(x) + g(x)) == Sum(n, f) + Sum(n, g)
 {
 }
 
-lemma {:induction false} PrettyBasicBetaReduction(n: nat, g: (int,int) -> int, i: int)
+lemma {:induction false} PrettyBasicBetaReduction(n: nat, g: (int,int) ~> int, i: int)
   requires Total2(g)
   ensures (x => Sum(n, y => g(x,y)))(i) == Sum(n, y => g(i,y))
 {
@@ -78,20 +78,20 @@ lemma {:induction false} PrettyBasicBetaReduction(n: nat, g: (int,int) -> int, i
   }
 }
 
-lemma BetaReduction0(n: nat, g: (int,int) -> int, i: int)
+lemma BetaReduction0(n: nat, g: (int,int) ~> int, i: int)
   requires Total2(g)
   ensures (x => Sum(n, y => g(x,y)))(i) == Sum(n, y => g(i,y))
 {
   // automatic proof by induction on n
 }
 
-lemma BetaReduction1(n': nat, g: (int,int) -> int, i: int)
+lemma BetaReduction1(n': nat, g: (int,int) ~> int, i: int)
   requires Total2(g)
   ensures g(i,n') + Sum(n', y => g(i,y)) == (x => g(x,n') + Sum(n', y => g(x,y)))(i);
 {
 }
 
-lemma BetaReductionInside(n': nat, g: (int,int) -> int)
+lemma BetaReductionInside(n': nat, g: (int,int) ~> int)
   requires Total2(g)
   ensures Sum(n', x => g(x,n') + Sum(n', y => g(x,y)))
        == Sum(n', x => (w => g(w,n'))(x) + (w => Sum(n', y => g(w,y)))(x))
@@ -106,7 +106,7 @@ lemma BetaReductionInside(n': nat, g: (int,int) -> int)
   Exchange(n', x => g(x,n') + Sum(n', y => g(x,y)), x => (w => g(w,n'))(x) + (w => Sum(n', y => g(w,y)))(x));
 }
 
-lemma L(n: nat, n': nat, g: (int, int) -> int)
+lemma L(n: nat, n': nat, g: (int, int) ~> int)
   requires Total2(g) && n == n' + 1
   ensures Sum(n, x => Sum(n, y => g(x,y)))
        == Sum(n', x => Sum(n', y => g(x,y))) + Sum(n', x => g(x,n')) + Sum(n', y => g(n',y)) + g(n',n')
@@ -154,12 +154,12 @@ lemma L(n: nat, n': nat, g: (int, int) -> int)
   }
 }
 
-lemma Commute(n: nat, g: (int,int) -> int)
+lemma Commute(n: nat, g: (int,int) ~> int)
   requires Total2(g)
   ensures Sum(n, x => Sum(n, y => g(x,y))) == Sum(n, x => Sum(n, y => g(y,x)))
 // TODO
   
-lemma CommuteSum(n: nat, g: (int,int) -> int)
+lemma CommuteSum(n: nat, g: (int,int) ~> int)
   requires Total2(g)
   ensures Sum(n, x => Sum(n, y => g(x,y))) == Sum(n, y => Sum(n, x => g(x,y)))
 // TODO
